$$
D(E(M))=M
$$

$$
E(D(M))=M
$$

$$
Y=f_k(X) 
$$

$$
X=f_k^{-1}(Y)
$$

$$
X=f_k^{-1}(Y)
$$

$$
C \equiv E(M) \equiv M^e \pmod n
$$

$$
M\equiv D(C) \equiv C^d \pmod n
$$

$$
n = p \cdot q
$$

$$
gcd(\phi(n), e)=1
$$

$$
\phi(n)=\phi(p\cdot q)=(p-1)\cdot(q-1)
$$

$$
ed\equiv1 \pmod {\phi(n)}
$$

$$
d\equiv e^{-1} \pmod {\phi(n)}
$$

$$
D(E(M))=M^{e^d}=M^{ed} \pmod n=M
$$

$$
M^{k\phi(n)+1} \pmod n=M^{k(p-1)(q-1)+1} \pmod n=M
$$

$$
M^{k(p-1)(q-1) + 1} \pmod p = M \pmod p
$$

$$
\begin{aligned}
M^{k(p-1)(q-1)+1} \pmod p&=[(M)M^{k(p-1)(q-1)}]\pmod p\\
&=[(M)(M^{(p-1)k(q-1)})] \pmod p\\
&=[(M)(M^{\phi(p)})^{k(q-1)}] \pmod p\\
&=(M \pmod p) \times [(M^{\phi(p)}) \pmod p]^{k(q-1)}\\
&=(M \pmod p) \times (1)^{k(q-1)}\\
&=M \pmod p
\end{aligned}
$$

$$
M^{k(p-1)(q-1) + 1} \pmod n=M \pmod n
$$

$$
M^{k(p-1)(q-1) + 1} \pmod n-M \pmod n=0
$$

$$
[M^{k(p-1)(q-1) + 1}-M] \pmod n=0
$$

$$
[M^{k(p-1)(q-1) + 1}-M]=nr=(pq)r
$$

$$
[M^{k(p-1)(q-1) + 1}-M] \pmod p = 0\\
M^{k(p-1)(q-1) + 1}\pmod p=M \pmod p
$$

$$
[(a \mod n) \times (b \mod n)] = (a \times b) \pmod n
$$

$$
M^{\phi(p)} \mod p=1
$$

$$
M \mod p = 0
$$

$$
p=47\\
q=59\\
n=p \cdot q=47 \cdot 59=2773\ and \ d=157
$$

$$
\phi(n)
$$

$$
exp\sqrt{ln(n)\cdot ln(ln(n))}=n^{\sqrt{lnln(n)/ln(n)}}=(ln(n))^{\sqrt{ln(n)/ln(ln(n))}}
$$

$$
\begin{aligned}
\phi(2773)&=46\cdot57=2668\\
x_0&=2668, a_0=1,b_0=0,\\
x_1&=157,a_1=0,b_1=1,\\
x_2&=156,a_2=1,b_2=-16\\
x_3&=1,a_3=-1,b_3=17=e
\end{aligned}
$$

$$
920^{17}=M^{17}=((((M^2)^2)^2)^2) \cdot M=948 \pmod {2773}
$$

